[Define: "x" as "{"A sequence $x_1, x_2, \ldots$"; "$x_1 = 1$"; "$x_{2k} = -x_k$"; "$x_{2k-1} = (-1)^{k+1} x_k$"; "for all $k \geq 1$"}"]
[Show: "$x_1 + x_2 + \cdots + x_n \geq 0$ for all $n \geq 1$"]
[Hint: "We start with some observations."]
[Have: "from the definition of $x_i$ it follows that for each positive integer $k$ we have $x_{4k-3} = x_{2k-1} = -x_{4k-2}$ and $x_{4k-1} = x_{4k} = -x_{2k} = x_k$." by "from the definition of $x_i$"]
[Define: "$S_n$" as ""$S_n = \sum_{i=1}^n x_i$""]
[Have: "$S_{4k} = \sum_{i=1}^k ((x_{4k-3} + x_{4k-2}) + (x_{4k-1} + x_{4k})) = \sum_{i=1}^k (0 + 2x_k) = 2S_k$"]
[Have: "$S_{4k+2} = S_{4k} + (x_{4k+1} + x_{4k+2}) = S_{4k}$"]
[Have: "$S_n = \sum_{i=1}^n x_i \equiv \sum_{i=1}^n 1 = n \ (\text{mod} \ 2)$"]
[Hint: "Now we prove by induction on $k$ that $S_i \geq 0$ for all $i \leq 4k$."]
[Have: "The base case is valid since $x_1 = x_3 = x_4 = 1, x_2 = -1$."]
[Hint: "For the induction step"]
[Assume: "$S_i \geq 0$ for all $i \leq 4k$"]
[Have: "$S_{4k+4} = 2S_{k+1} \geq 0, \quad S_{4k+2} = S_{4k} \geq 0, \quad S_{4k+3} = S_{4k+2} + x_{4k+3} = \frac{S_{4k+2} + S_{4k+4}}{2} \geq 0.$" by "Using the relations (1)-(3)"]
[Show: "$S_{4k+1} \geq 0$"]
[Assume: "$k$ is odd"]
[Have: "$S_{4k} = 2S_k \geq 0$; since $k$ is odd, $S_k$ is odd as well, so we have $S_{4k} \geq 2$ and hence $S_{4k+1} = S_{4k} + x_{4k+1} \geq 1$."]
[Assume: "$k$ is even"]
[Have: "$x_{4k+1} = x_{2k+1} = x_{k+1}$"]
[Have: "$S_{4k+1} = S_{4k} + x_{4k+1} = 2S_k + x_{k+1} = S_k + S_{k+1} \geq 0$"]
[Hint: "The step is proved."]