[Show: "For all positive integers $n>2$, $n!\mid \left(\prod\limits_{p<q\leqslant n,}(p+q)\right)$ only holds for $n=7$."]
[Assume: "$n$ satisfies $n!\mid \prod\limits_{p<q\leq n}(p+q)$"]
[Fix: {p_1,\ldots,p_m} st "let $2=p_1<p_2<\cdots<p_m\leq n$ be the primes in $1,2,\cdots,n$"]
[Have: "Each such prime divides $n!$."]
[Have: "$p_m\mid p_i+p_j$ for some $p_i<p_j\leqslant n.$"]
[Have: "$0<\frac{p_i+p_j}{p_m}<2$"]
[Have: "$p_m=p_i+p_j$ which implies $m\geqslant3,p_i=2$ and $p_m=2+p_j=2+p_{m-1}.$"]
[Have: "$p_{m-1}\mid p_{k}+p_{l}$ for some $p_{k}<p_{l}\leqslant n.$"]
[Have: "$0<\dfrac{p_l+p_k}{p_{m-1}}\leqslant\dfrac{p_m+p_{m-1}}{p_{m-1}}=\dfrac{2p_{m-1}+2}{p_{m-1}}<3$"]
[Have: "either $p_m-1=p_l+p_k$ or $2p_{m-1}=p_l+p_k.$"]
[Have: "As above, the former case gives $p_m-1=2+p_{m-2}.$"]
[Have: "If $2p_{m-1}=p_{l}+p_{k}$,then $p_{m-1}<p_{k}$, so $k=m$ and $$2p_{m-1}=p_l+p_{m-1}+2\Rightarrow p_{m-1}=p_l+2=p_{m-2}+2.$$"]
[Have: "Either way, $p_{m-2} > 2$ and 3 divides one of $p_{m-2}, p_{m-1} = p_{m-2} + 2$ and $p_m = p_{m-2} + 4$. "]
[Have: "This implies $p_{m-2} = 3$ and thus $p_m = 7$, giving $7 \leq n < 11$. "]
[Have: "$7! \mid \prod_{p < q \leq 7} (p + q)$"]
[Have: "$8! \nmid \prod_{p < q \leq 7} (p + q)$"]
[Have: "$9!,10! \nmid \prod_{p < q \leq 7} (p + q)$"]