[Fix: {n, x, y} st {"n is a positive integer"; "x and y are positive real numbers"; "x^n + y^n = 1"}]
[Show: "( \sum_{k=1}^n \frac{1 + x^{2k}}{1 + x^{4k}} ) ( \sum_{k=1}^n \frac{1 + y^{2k}}{1 + y^{4k}} ) < \frac{1}{(1 - x)(1 - y)}"]
[Fix: {t} st "t \in (0,1)"]
[Have: "\frac{1 + t^2}{1 + t^4} = \frac{1}{t} - \frac{(1 - t)(1 - t^3)}{t(1 + t^4)} < \frac{1}{t}"]
[Hint: "Substituting t = x^k and t = y^k"]
[Have: "0 < \sum_{k=1}^n \frac{1 + x^{2k}}{1 + x^{4k}} < \sum_{k=1}^n \frac{1}{x^k} = \frac{1 - x^n}{x^n (1 - x)}"]
[Have: "0 < \sum_{k=1}^n \frac{1 + y^{2k}}{1 + y^{4k}} < \sum_{k=1}^n \frac{1}{y^k} = \frac{1 - y^n}{y^n (1 - y)}"]
[Have: {"1 - y^n = x^n"; "1 - x^n = y^n"}]
[Have: "\frac{1 - x^n}{x^n (1 - x)} = \frac{y^n}{x^n (1 - x)}, \quad \frac{1 - y^n}{y^n (1 - y)} = \frac{x^n}{y^n (1 - y)}"]
[Have: "( \sum_{k=1}^n \frac{1 + x^{2k}}{1 + x^{4k}} ) ( \sum_{k=1}^n \frac{1 + y^{2k}}{1 + y^{4k}} ) < \frac{y^n}{x^n (1 - x)} \cdot \frac{x^n}{y^n (1 - y)} = \frac{1}{(1 - x)(1 - y)}"]