[Show: "Let $a_0,a_1,a_2,\ldots$ be a sequence of positive integers with $\gcd(a_i,a_{i+1})>a_{i-1}$ for all $i\ge 0$"]
[Fix: {a} st {"$a_0,a_1,a_2,\ldots$ are positive integers"; "for all $i\ge 0$, $\gcd(a_i,a_{i+1})>a_{i-1}$"}]
[Show: "$a_n \ge 2^n$ for all $n\ge 0$"]
[Have: "$a_i \ge \gcd(a_i,a_{i+1})>a_{i-1}$"]
[Have: "the sequence $\{a_i\}$ is strictly increasing" by "$a_i \ge \gcd(a_i,a_{i+1})>a_{i-1}$"]
[Have: "$a_0\ge 1,\ a_1\ge 2$"]
[Have: "for each $i\ge 1$, $a_{i+1}-a_i\ge \gcd(a_i,a_{i+1})>a_{i-1}$"]
[Have: "$a_{i+1}\ge a_i+a_{i-1}+1$" by "consequently"]
[Have: "$a_2\ge 4$ and $a_3\ge 7$"]
[Assume: "$a_3=7$"]
[Have: "$\gcd(a_2,a_3)=\gcd(4,7)>a_1=2$" by "equalities in the previous estimates"]
[Have: "contradiction"]
[Have: "$a_3\ge 8$"]
[Have: "the result is valid for $n=0,1,2,3$"]
[Hint: "These are the base cases for a proof by induction."]
[Fix: {n} st "$n\ge 3$"]
[Assume: "$a_i\ge 2^i$ for $i=0,1,\ldots,n$"]
[Show: "$a_{n+1}\ge 2^{n+1}$"]
[Define: "d" as ""$\gcd(a_n,a_{n+1})=d$""]
[Have: "$d>a_{n-1}$"]
[Hint: "The induction claim is reached immediately in the following cases:"]
[Assume: "$a_{n+1}\ge 4d$"]
[Have: "$a_{n+1}>4a_{n-1}\ge 4\cdot 2^{n-1}=2^{n+1}$"]
[Assume: "$a_n\ge 3d$"]
[Have: "$a_{n+1}\ge a_n+d\ge 4d>4a_{n-1}\ge 4\cdot 2^{n-1}=2^{n+1}$"]
[Assume: "$a_n=d$"]
[Have: "$a_{n+1}\ge a_n+d=2a_n\ge 2\cdot 2^n=2^{n+1}$"]
[Assume: {"$a_n=2d$"; "$a_{n+1}=3d$"}]
[Have: "$a_{n+1}=\tfrac{3}{2}a_n$"]
[Define: "d'" as ""$\gcd(a_{n-1},a_n)=d'$""]
[Have: "$d'>a_{n-2}$"]
[Fix: {m} st {"$a_n=md'$"; "$m$ is an integer"}]
[Have: "$m\ge 3$" by {"$d'\le a_{n-1}<d$"; "$a_n=2d$"}]
[Have: "$a_{n-1}<d=\tfrac{1}{2}md'$, $a_{n+1}=\tfrac{3}{2}md'$"]
[Hint: "Again we single out the cases which imply the induction claim immediately:"]
[Assume: "$m\ge 6$"]
[Have: "$a_{n+1}=\tfrac{3}{2}md'\ge 9d'>9a_{n-2}\ge 9\cdot 2^{n-2}=2^{n+1}$"]
[Assume: "$3\le m\le 4$"]
[Have: "$a_{n-1}<\tfrac{1}{2}\cdot 4d'$, and hence $a_{n-1}=d'$, $a_{n+1}=\tfrac{3}{2}ma_{n-1}\ge \tfrac{3}{2}\cdot 3a_{n-1}=\tfrac{9}{2}\cdot 2^{n-2}=2^{n+1}$"]
[Assume: "$m=5$"]
[Have: "$a_n=5d'$, $a_{n+1}=\tfrac{15}{2}d'$, and $a_{n-1}<d=\tfrac{5}{2}d'$"]
[Have: "$a_{n-1}$ is either $d'$ or $2d'$"]
[Have: "$a_n\ge 2d'$"]
[Hint: "The same pattern repeats once more."]
[Define: "d''" as ""$\gcd(a_{n-2},a_{n-1})=d''$""]
[Have: "$d''>a_{n-3}$"]
[Fix: {m'} st {"$2d'=m'd''$"; "$m'$ is an integer"}]
[Have: "$m'\ge 3$" by "$d''<a_{n-2}<d'$"]
[Have: "$a_{n-2}<d'=\tfrac{1}{2}m'd''$, $a_{n+1}=\tfrac{15}{4}m'd''$"]
[Hint: "As before, we consider the cases:"]
[Assume: "$m'\ge 5$"]
[Have: "$a_{n+1}=\tfrac{15}{4}m'd''\ge \tfrac{75}{4}d''>\tfrac{75}{4}a_{n-3}\ge \tfrac{75}{4}\cdot 2^{n-3}>2^{n+1}$"]
[Assume: "$3\le m'\le 4$"]
[Have: "$a_{n-2}<\tfrac{1}{2}\cdot 4d''$, and hence $a_{n-2}=d''$, $a_{n+1}=\tfrac{15}{4}m'a_{n-2}=\tfrac{15}{4}\cdot 3a_{n-2}\ge \tfrac{45}{4}\cdot 2^{n-2}>2^{n+1}$"]
[Hint: "Both of them have produced the induction claim. But now there are no cases left."]
[Have: "$a_{n+1}\ge 2^{n+1}$"]
[Have: "$a_n\ge 2^n$ holds for all $n$"]