[Fix: {f, g, x_0, u_0} st {"u=g(x) 在 x_0 处连续"; "g(x_0)=u_0"; "y=f(u) 在 u_0 处连续"}]
{
    [Show: "y=f(g(x)) 在 x_0 处连续"]
    {
        [Fix: {ε} st "ε>0"]
        {
            [Have: "存在 η>0 使得当 |u-u_0|<η 时, |f(u)-f(u_0)|<ε" by "lim_{u→u_0} f(u)=f(u_0)"]
            [Fix: {η} st {"η>0"; "当 |u-u_0|<η 时, |f(u)-f(u_0)|<ε"}]
            {
                [Have: "存在 δ>0 使得当 |x-x_0|<δ 时, |g(x)-u_0|<η" by "lim_{x→x_0} g(x)=u_0"]
                [Fix: {δ} st {"δ>0"; "当 |x-x_0|<δ 时, |g(x)-u_0|<η"}]
                {
                    [Have: "当 |x-x_0|<δ 时, |f(g(x))-f(g(x_0))|<ε" by {"|g(x)-u_0|<η"; "|f(u)-f(u_0)|<ε 当 |u-u_0|<η"}]
                }
            }
            [Have: "lim_{x→x_0} f(g(x)) = f(g(x_0))" by "对任意 ε>0 存在 δ>0 使 |x-x_0|<δ ⇒ |f(g(x))-f(g(x_0))|<ε"]
        }
    }
}