求$\displaystyle\int \frac{4x^3 - 13x^2 + 3x + 8}{(x+1)(x-2)(x-1)^2} \, dx$

先将被积函数分解成简单分式之和。设：
$\displaystyle\frac{4x^3 - 13x^2 + 3x + 8}{(x+1)(x-2)(x-1)^2} = \frac{A}{x+1} + \frac{B}{x-2} + \frac{C}{x-1} + \frac{D}{(x-1)^2}.$

将右边通分后，两边的分子应该相等，所以：
$4x^3 - 13x^2 + 3x + 8 = A(x-2)(x-1)^2 + B(x+1)(x-1)^2 +$
$C(x+1)(x-2)(x-1) + D(x+1)(x-2).$
令 $x = -1$，得到 $A = 1$；
令 $x = 2$，得到 $B = -2$；
令 $x = 1$，得到 $D = -1$；
两边求导后再令 $x = 1$，得到 $C = 5$，
于是：
$\displaystyle\int \frac{4x^3 - 13x^2 + 3x + 8}{(x+1)(x-2)(x-1)^2} \, dx = \int \left[ \frac{1}{x+1} - \frac{2}{x-2} + \frac{5}{x-1} - \frac{1}{(x-1)^2} \right] \, dx$
计算得：
$$
= \ln |(x+1)(x-1)^5| - \ln |(x-2)^2| + \frac{1}{x-1} + C.
$$