Exercise 4.2.6 If $a^2 = 0$ in $R$, show that $ax + xa$ commutes with $a$.
Proof.
We need to show that
$$
a(a x+x a)=(a x+x a) a \text { for } a, x \in R .
$$
Now,
$$
\begin{gathered}
a(a x+x a)=a(a x)+a(x a) \\
=a^2 x+a x a \\
=0+a x a=a x a .
\end{gathered}
$$
Again,
$$
\begin{gathered}
(a x+x a) a=(a x) a+(x a) a \\
=a x a+x a^2 \\
=a x a+0=a x a .
\end{gathered}
$$
It follows that,
$$
a(a x+x a)=(a x+x a) a, \text { for } x, a \in R .
$$
This shows that $a x+x a$ commutes with $a$. This completes the proof.
Qed.