[Find: "\displaystyle\int \frac{4x^3 - 13x^2 + 3x + 8}{(x+1)(x-2)(x-1)^2} \, dx"]
[Perform: "分解成简单分式之和" to "$\frac{4x^3 - 13x^2 + 3x + 8}{(x+1)(x-2)(x-1)^2}$"]
[Fix: {A,B,C,D} such that "$\frac{4x^3 - 13x^2 + 3x + 8}{(x+1)(x-2)(x-1)^2} = \frac{A}{x+1} + \frac{B}{x-2} + \frac{C}{x-1} + \frac{D}{(x-1)^2}$"]
[Have: "$4x^3 - 13x^2 + 3x + 8 = A(x-2)(x-1)^2 + B(x+1)(x-1)^2 + C(x+1)(x-2)(x-1) + D(x+1)(x-2)$" by "将右边通分后，两边的分子应该相等"]
[Have: "$A = 1$" by "令$x=-1$"]
[Have: "$B = -2$" by "令$x=2$"]
[Have: "$D = -1$" by "令$x=1$"]
[Have: "$C = 5$" by "两边求导后再令$x=1$"]
[Have: "$\displaystyle\int \frac{4x^3 - 13x^2 + 3x + 8}{(x+1)(x-2)(x-1)^2} \, dx = \int \left[ \frac{1}{x+1} - \frac{2}{x-2} + \frac{5}{x-1} - \frac{1}{(x-1)^2} \right] \, dx$"]
[Have: "$\displaystyle\int \frac{4x^3 - 13x^2 + 3x + 8}{(x+1)(x-2)(x-1)^2} \, dx = = \ln |(x+1)(x-1)^5| - \ln |(x-2)^2| + \frac{1}{x-1} + C$"]