[Assume: "R is an equivalence relation on \mathbb{R}"]
[Show: "S_2 defined as S_2 = \left\{ ([a]_R, [b]_R) \mid \exists a' \in [a]_R, b' \in [b]_R, a' - b' = \frac{1}{2} \right\} \cup \{([a]_R, [a]_R) \mid a \in \mathbb{R} \}"]
[Show: "S_2 is an equivalence relation"]
[Show: "S_2 is reflexive"]
[Show: "For all [a]_R, ([a]_R, [a]_R) \in S_2"]
[Have: "For all [a]_R, ([a]_R, [a]_R) \in S_2" by "By definition of S_2"]
[Show: "S_2 is symmetric"]
[Show: "If ([a]_R, [b]_R) \in S_2, then ([b]_R, [a]_R) \in S_2"]
[Assume: "([a]_R, [b]_R) \in S_2"]
[Show: "There exist a' \in [a]_R, b' \in [b]_R such that a' - b' = \frac{1}{2}"]
[Show: "Let b'' = b' + 1 \in [b]_R"]
[Show: "b'' - a' = \frac{1}{2}"]
[Show: "([b]_R, [a]_R) \in S_2"]
[Show: "S_2 is transitive"]
[Show: "If ([a]_R, [b]_R) \in S_2 and ([b]_R, [c]_R) \in S_2, then ([a]_R, [c]_R) \in S_2"]
[Assume: {"([a]_R, [b]_R) \in S_2"; "([b]_R, [c]_R) \in S_2"}]
[Show: "There exists a' \in [a]_R, b_1 \in [b]_R with a' - b_1 = \frac{1}{2}"]
[Show: "There exists b_2 \in [b]_R, c' \in [c]_R with b_2 - c' = \frac{1}{2}"]
[Show: "Since b_1, b_2 \in [b]_R, b_1 - b_2 = k \in \mathbb{Z}"]
[Show: "Let c'' = c' + k \in [c]_R"]
[Show: "a' - c'' = (a' - b_1) + (b_1 - c'') = \frac{1}{2} + (b_1 - (c' + k)) = \frac{1}{2} - \frac{1}{2} = 0"]
[Show: "[a]_R = [c]_R"]
[Show: "([a]_R, [c]_R) \in S_2"]